src/tls/Negotiation.Writers.LayeredEffects.fst
@@ -47,4 +47,173 @@ let write_obfuscate_age'
   LWP.append LWP.parse_u32 LowParse.Low.Int.write_u32 obfuscated_age;
   LWP.valid_synth _ _ _ _ _ Aux.valid_pskIdentity_intro
 
-#pop-options
+[@@expect_failure] // FIXME: WHY WHY WHY?
+inline_for_extraction
+noextract
+let write_clientHelloExtension_CHE_early_data
+  (#inv: LWP.memory_invariant)
+  ()
+: LWP.EWrite
+    unit
+    LWP.emp
+    Parsers.ClientHelloExtension.lwp_clientHelloExtension
+    (fun _ -> True)
+    (fun _ _ out -> out == Parsers.ClientHelloExtension.CHE_early_data ())
+    (fun _ -> True)
+    inv
+=
+  LWP.start Parsers.ExtensionType.lwp_extensionType
+  Parsers.ExtensionType.extensionType_writer Parsers.ExtensionType.Early_data;
+  LWP.frame _ _ _ _ _ _ _ (fun _ ->
+    LWP.parse_vldata_intro_ho
+      LWP.emp 0ul 65535ul _ _ _ (wret #inv)
+  );
+  LWP.wfailwith "abc"
+
+[@@expect_failure] // FIXME: WHY WHY WHY?
+inline_for_extraction
+noextract
+let write_clientHelloExtension_CHE_early_data
+  (#inv: LWP.memory_invariant)
+  ()
+: LWP.EWrite
+    unit
+    LWP.emp
+    Parsers.ClientHelloExtension.lwp_clientHelloExtension
+    (fun _ -> True)
+    (fun _ _ out -> out == Parsers.ClientHelloExtension.CHE_early_data ())
+    (fun _ -> True)
+    inv
+=
+  LWP.start Parsers.ExtensionType.lwp_extensionType
+  Parsers.ExtensionType.extensionType_writer Parsers.ExtensionType.Early_data;
+  LWP.frame _ _ _ _ _ _ _ (fun _ ->
+    LWP.parse_vldata_intro_ho
+      LWP.emp 0ul 65535ul _ _ _ (wret #inv);
+    LWP.valid_synth _ _ _ _ _ Aux.valid_clientHelloExtension_CHE_early_data_intro
+  );
+  LWP.valid_synth _ _ _ _ _ Aux2.valid_synth_constr_clientHelloExtension_CHE_early_data
+
+let wret #inv () : LWP.Write unit LWP.emp LWP.emp (fun _ -> True) (fun _ _ _ -> True) inv = ()
+
+
+inline_for_extraction
+let parse_vldata_intro_ho
+  (#inv: LWP.memory_invariant)
+  (p: LWP.parser)
+  (min: U32.t)
+  (max: U32.t { U32.v min <= U32.v max /\ U32.v max > 0 })
+  (pre: LWP.pre_t LWP.emp)
+  (post: LWP.post_t unit LWP.emp p pre)
+  (post_err: LWP.post_err_t LWP.emp pre)
+  ($f: (unit -> LWP.EWrite unit LWP.emp p pre post post_err inv))
+  ()
+: LWP.EWrite unit LWP.emp (LWP.parse_vldata p min max)
+    (fun _ ->
+      pre () /\
+      begin match LWP.destr_repr_spec _ _ _ _ _ _ _ f () with
+      | LWP.Correct (_, v) ->
+        post () () v ==> (U32.v min <= LWP.size p v /\ LWP.size p v <= U32.v max)
+      | _ -> True
+      end
+    )
+    (fun _ _ vout ->
+      pre () /\
+      begin match LWP.destr_repr_spec _ _ _ _ _ _ _ f () with
+      | LWP.Correct (_, v) ->
+        post () () v /\
+        (vout <: dfst p) == v
+      | _ -> False
+      end
+    )
+    (fun vin ->
+      post_err ()
+    )
+    inv
+= LWP.parse_vldata_intro_ho p min max pre post post_err f
+
+inline_for_extraction
+noextract
+let write_clientHelloExtension_CHE_early_data
+  (#inv: LWP.memory_invariant)
+  ()
+: LWP.Write
+    unit
+    LWP.emp
+    Parsers.ClientHelloExtension.lwp_clientHelloExtension
+    (fun _ -> True)
+    (fun _ _ out -> out == Parsers.ClientHelloExtension.CHE_early_data ())
+    inv
+=
+  LWP.start Parsers.ExtensionType.lwp_extensionType
+    Parsers.ExtensionType.extensionType_writer Parsers.ExtensionType.Early_data;
+  LWP.frame _ _ _ _ _ _ _ (
+    parse_vldata_intro_ho
+      LWP.emp 0ul 65535ul _ _ _ (wret #inv)
+  );
+  LWP.valid_synth _ _ _ _ _
+    (LWP.valid_synth_star_compat_l
+      _ _ _ _ _
+      Aux.valid_clientHelloExtension_CHE_early_data_intro
+    );
+  LWP.valid_synth _ _ _ _ _ Aux2.valid_synth_constr_clientHelloExtension_CHE_early_data
+
+module L = FStar.List.Tot
+
+[@@expect_failure] // FIXME: WHY WHY WHY?
+let write_final_extensions
+  (#inv: LWP.memory_invariant)
+  (cfg: LWP.ptr Parsers.MiTLSConfig.lwp_miTLSConfig inv)
+  (edi: bool)
+  (lri: LWP.lptr Parsers.ResumeInfo13.lwp_resumeInfo13 inv)
+  (now: U32.t)
+  (max: U32.t { U32.v max > 0 })
+: LWP.EWrite
+    unit
+    (LWP.parse_vllist Parsers.ClientHelloExtension.lwp_clientHelloExtension 0ul max)
+    (LWP.parse_vllist Parsers.ClientHelloExtension.lwp_clientHelloExtension 0ul max)
+    (fun _ -> True)
+    (fun vin _ vout ->
+      match final_extensions_new (LWP.deref_spec cfg) edi (LWP.deref_list_spec lri) now with
+      | TLS.Result.Correct l -> (vout <: list Parsers.ClientHelloExtension.clientHelloExtension) == (vin `L.append` l)
+      | _ -> False
+    )
+    (fun vin ->
+      True
+(*
+      match final_extensions_new (LWP.deref_spec cfg) edi (LWP.deref_list_spec lri) with
+      | Correct l -> LWP.list_size Parsers.ClientHelloExtension.lwp_clientHelloExtension vin + LWP.list_size Parsers.ClientHelloExtension.lwp_clientHelloExtension l > U32.v max
+      | _ -> True
+*)
+    )
+    inv
+= let vin = LWP.get_state () in
+  let max_version = LWP.deref Parsers.ProtocolVersion.protocolVersion_reader (Parsers.KnownProtocolVersion.lwp_knownProtocolVersion_accessor_tag (Parsers.MiTLSConfig.lwp_accessor_miTLSConfig_max_version cfg)) in
+  match max_version with
+  | TLS_1p3 ->
+    let allow_psk_resumption = LWP.list_exists allow_psk_resumption_new (fun _ -> true) lri in
+    let allow_dhe_resumption = LWP.list_exists allow_dhe_resumption_new (fun _ -> true) lri in
+    if allow_psk_resumption || allow_dhe_resumption
+    then
+      LWP.wfailwith "not implemented" 
+    else begin
+      LWP.parse_vllist_snoc_ho Parsers.ClientHelloExtension.lwp_clientHelloExtension 0ul max _ _ _ (
+        Aux2.constr_clientHelloExtension_CHE_psk_key_exchange_modes (
+          parse_vldata_intro_ho Parsers.PskKeyExchangeModes.lwp_pskKeyExchangeModes 0ul 65535ul _ _ _ (fun _ ->
+            let open Parsers.PskKeyExchangeMode in
+            LWP.parse_vllist_nil lwp_pskKeyExchangeMode 255ul;
+            LWP.parse_vllist_snoc_ho lwp_pskKeyExchangeMode 0ul 255ul _ _ _ (fun _ ->
+              LWP.start lwp_pskKeyExchangeMode pskKeyExchangeMode_writer Psk_ke
+            );
+            LWP.parse_vllist_snoc_ho lwp_pskKeyExchangeMode 0ul 255ul _ _ _ (fun _ ->
+              LWP.start lwp_pskKeyExchangeMode pskKeyExchangeMode_writer Psk_dhe_ke
+            );
+            LWP.parse_vllist_recast _ _ _ 1ul 255ul;
+            LWP.valid_synth _ _ _ _ _
+              Aux.valid_synth_pskKeyExchangeModes_intro
+          )
+        )
+      )
+    end
+  | _ ->
+    L.append_l_nil (Ghost.reveal vin <: list Parsers.ClientHelloExtension.clientHelloExtension)
